Verified initialization function for a plausible new Scheduler invariant

platform/Scheduler.v
@@ -1,6 +1,25 @@
-Require Import AutoSep Malloc Bags ThreadQueues.
+Require Import AutoSep Malloc Bags ThreadQueues SinglyLinkedList.
 Import W_Bag.
 Export AutoSep Malloc W_Bag.
+
+Lemma equiv_empty : forall ls, empty %= bagify ls
+  -> ls = nil.
+  unfold bagify; destruct ls; simpl; intuition.
+  eapply equiv_symm in H; eapply equiv_trans in H; [ | eapply equiv_symm; eapply add_something ].
+  elimtype False.
+  generalize dependent (fold_left add ls empty); intros.
+  bags.
+  specialize (H a).
+  destruct (W_Key.eq_dec a a); congruence.
+Qed.
+
+Theorem starB_empty_fwd : forall P, starB P empty ===> Emp.
+  unfold starB; intros; intro.
+  apply himp_ex_p; intros.
+  apply himp_star_pure_c; intro H.
+  apply equiv_empty in H; subst.
+  reflexivity.
+Qed.
 
 
 Module Type S.
@@ -13,71 +32,201 @@ Module Make(M : S).
 Import M.
 
 Module M''.
-  Definition world := unit.
+  Definition world := bag.
 
-  Definition evolve (_ _ : unit) := True.
+  Definition evolve : bag -> bag -> Prop := incl.
 
   Theorem evolve_refl : forall w, evolve w w.
-    red; auto.
+    red; bags.
   Qed.
 
   Theorem evolve_trans : forall w1 w2 w3, evolve w1 w2 -> evolve w2 w3 -> evolve w1 w3.
-    red; auto.
+    unfold evolve in *; bags.
   Qed.
 
   Open Scope Sep_scope.
 
-  Definition globalInv (ts : bag) (_ : world) : HProp :=
-    Ex q, [| q %in ts |] * globalSched =*> q * globalInv.
+  Definition globalInv (ts : bag) (w : world) : HProp :=
+    (* The scheduler entry point *)
+    Ex p, globalSched =*> p
+    * Ex ready, Ex free, Ex wait, Ex waitLen, (p ==*> ready, free, wait, waitLen)
+
+    (* The ready queue is a valid thread queue, for threads ready to run immediately. *)
+    * [| ready %in ts |]
+
+    (* The free list stores available file pointers. *)
+    * Ex freeL, sll freeL free * [| List.Forall (fun p => p %in w) freeL |]
+
+    (* Each available file pointer stores a record of a file descriptor and input/output thread queues. *)
+    * starB (fun p => Ex fd, Ex inq, Ex outq, (p ==*> fd, inq, outq) * [| inq %in ts |] * [| outq %in ts |]) w
+
+    (* There is an array correspoinding to outstanding declare() calls, mapping each to a queue that should be poked when its event is enabled. *)
+    * Ex waitL, array waitL wait * [| List.Forall (fun p => p = $0 \/ p %in ts) waitL |]
+      * [| length waitL = wordToNat waitLen |]
+      * [| (length waitL >= 2)%nat |] * [| wait <> 0 |] * [| freeable wait (length waitL) |]
+
+    (* Finally, the application-specific global invariant holds. *)
+    * globalInv.
 End M''.
 
 Module Q' := ThreadQueues.Make(M'').
 Import M'' Q'.
 Export M'' Q'.
 
-Module Type SCHED.
-  Parameter sched : HProp.
+Definition allIn (b : bag) := List.Forall (fun p => p %in b).
+Definition allInOrZero (b : bag) := List.Forall (fun p => p = $0 \/ p %in b).
 
-  Axiom sched_fwd : sched ===> Ex ts, Ex q, [| q %in ts |] * globalSched =*> q * tqs ts tt.
-  Axiom sched_bwd : (Ex ts, Ex q, [| q %in ts |] * globalSched =*> q * tqs ts tt) ===> sched.
+Module Type SCHED.
+  Parameter sched : bag -> HProp.
+  (* Parameter is available file pointers. *)
+
+  Parameter files : bag -> bag -> HProp.
+
+  Axiom sched_fwd : forall fs, sched fs ===>
+    Ex ts, Ex p, globalSched =*> p
+    * Ex ready, Ex free, Ex wait, Ex waitLen, (p ==*> ready, free, wait, waitLen)
+    * [| ready %in ts |]
+    * Ex freeL, sll freeL free * [| allIn fs freeL |]
+    * files ts fs
+    * Ex waitL, array waitL wait * [| allInOrZero ts waitL |] * [| length waitL = wordToNat waitLen |]
+      * [| (length waitL >= 2)%nat |] * [| wait <> 0 |] * [| freeable wait (length waitL) |]
+    * tqs ts fs.
+
+  Axiom sched_bwd : forall fs,
+    (Ex ts, Ex p, globalSched =*> p
+     * Ex ready, Ex free, Ex wait, Ex waitLen, (p ==*> ready, free, wait, waitLen)
+     * [| ready %in ts |]
+     * Ex freeL, sll freeL free * [| allIn fs freeL |]
+     * files ts fs
+     * Ex waitL, array waitL wait * [| allInOrZero ts waitL |] * [| length waitL = wordToNat waitLen |]
+       * [| (length waitL >= 2)%nat |] * [| wait <> 0 |] * [| freeable wait (length waitL) |]
+     * tqs ts fs)
+    ===> sched fs.
+
+  Axiom files_empty_fwd : forall ts, files ts empty ===> Emp.
+  Axiom files_empty_bwd : forall ts, Emp ===> files ts empty.
 End SCHED.
 
 Module Sched : SCHED.
   Open Scope Sep_scope.
 
-  Definition sched := Ex ts, Ex q, [| q %in ts |] * globalSched =*> q * tqs ts tt.
+  Definition files (ts : bag) : bag -> HProp :=
+    starB (fun p => Ex fd, Ex inq, Ex outq, (p ==*> fd, inq, outq) * [| inq %in ts |] * [| outq %in ts |]).
 
-  Theorem sched_fwd : sched ===> Ex ts, Ex q, [| q %in ts |] * globalSched =*> q * tqs ts tt.
-    unfold sched; sepLemma.
+  Definition sched fs :=
+    Ex ts, Ex p, globalSched =*> p
+    * Ex ready, Ex free, Ex wait, Ex waitLen, (p ==*> ready, free, wait, waitLen)
+    * [| ready %in ts |]
+    * Ex freeL, sll freeL free * [| allIn fs freeL |]
+    * files ts fs
+    * Ex waitL, array waitL wait * [| allInOrZero ts waitL |] * [| length waitL = wordToNat waitLen |]
+      * [| (length waitL >= 2)%nat |] * [| wait <> 0 |] * [| freeable wait (length waitL) |]
+    * tqs ts fs.
+
+  Theorem sched_fwd : forall fs, sched fs ===>
+    Ex ts, Ex p, globalSched =*> p
+    * Ex ready, Ex free, Ex wait, Ex waitLen, (p ==*> ready, free, wait, waitLen)
+    * [| ready %in ts |]
+    * Ex freeL, sll freeL free * [| allIn fs freeL |]
+    * files ts fs
+    * Ex waitL, array waitL wait * [| allInOrZero ts waitL |] * [| length waitL = wordToNat waitLen |]
+      * [| (length waitL >= 2)%nat |] * [| wait <> 0 |] * [| freeable wait (length waitL) |]
+    * tqs ts fs.
+    intros; apply Himp_refl.
   Qed.
 
-  Theorem sched_bwd : (Ex ts, Ex q, [| q %in ts |] * globalSched =*> q * tqs ts tt) ===> sched.
-    unfold sched; sepLemma.
+  Theorem sched_bwd : forall fs,
+    (Ex ts, Ex p, globalSched =*> p
+     * Ex ready, Ex free, Ex wait, Ex waitLen, (p ==*> ready, free, wait, waitLen)
+     * [| ready %in ts |]
+     * Ex freeL, sll freeL free * [| allIn fs freeL |]
+     * files ts fs
+     * Ex waitL, array waitL wait * [| allInOrZero ts waitL |] * [| length waitL = wordToNat waitLen |]
+       * [| (length waitL >= 2)%nat |] * [| wait <> 0 |] * [| freeable wait (length waitL) |]
+     * tqs ts fs)
+     ===> sched fs.
+    intros; apply Himp_refl.
+  Qed.
+
+  Theorem files_empty_fwd : forall ts, files ts empty ===> Emp.
+    intros; apply starB_empty_fwd.
+  Qed.
+
+  Theorem files_empty_bwd : forall ts, Emp ===> files ts empty.
+    intros; apply starB_empty_bwd.
   Qed.
 End Sched.
 
 Import Sched.
 Export Sched.
 
+Lemma allocate_array' : forall p n offset,
+  allocated p offset n ===> Ex ls, [| length ls = n |] * array ls (p ^+ $(offset)).
+  induction n; simpl.
+
+  sepLemma.
+  instantiate (1 := nil); auto.
+  sepLemma.
+
+  intros; sepLemmaLhsOnly.
+  etransitivity; [ eapply himp_star_frame; [ apply IHn | reflexivity ] | ]; clear IHn.
+  sepLemmaLhsOnly.
+  apply himp_ex_c; exists (x :: x0).
+  sepLemma.
+  etransitivity; [ eapply himp_star_frame; [ apply ptsto32m'_in | reflexivity ] | ].
+  etransitivity; [ | apply ptsto32m'_out ].
+  simpl.
+  destruct offset; simpl.
+  replace (p ^+ natToW 0) with p by words; sepLemma.
+  etransitivity; [ | apply ptsto32m'_shift_base ].
+  instantiate (1 := 4); reflexivity.
+  auto.
+  replace (p ^+ natToW (S offset) ^+ $0) with (p ^+ natToW (S offset)) by words.
+  sepLemma.
+  etransitivity; [ | apply ptsto32m'_shift_base ].
+  instantiate (1 := 4).
+  rewrite <- wplus_assoc.
+  rewrite <- natToW_plus.
+  replace (S offset + 4) with (S (S (S (S (S offset))))) by omega.
+  reflexivity.
+  auto.
+Qed.
+
+Inductive make_array (sz : nat) : Prop := MakeArray.
+
+Hint Constructors make_array.
+
+Lemma allocate_array : forall p n,
+  make_array n
+  -> p =?> n ===> Ex ls, [| length ls = n |] * array ls p.
+  intros; eapply Himp_trans; [ apply allocate_array' | ].
+  replace (p ^+ $0) with p by words; apply Himp_refl.
+Qed.
+
+Theorem tqs_empty_bwd : forall w, Emp ===> tqs empty w.
+  intros; rewrite tqs_eq; apply tqs'_empty_bwd.
+Qed.
+
 Definition hints : TacPackage.
-  prepare sched_fwd sched_bwd.
+  prepare (sched_fwd, SinglyLinkedList.nil_fwd, SinglyLinkedList.cons_fwd, allocate_array, files_empty_fwd)
+  (sched_bwd, SinglyLinkedList.nil_bwd, SinglyLinkedList.cons_bwd, tqs_empty_bwd, files_empty_bwd).
 Defined.
 
 Definition starting (pc : W) (ss : nat) : HProp := fun s m =>
   (ExX (* pre *) : settings * state, Cptr pc #0
     /\ [| semp m |]
-    /\ Al st : settings * state, Al vs,
+    /\ Al st : settings * state, Al vs, Al fs,
       [| st#Sp <> 0 /\ freeable st#Sp (1 + ss) |]
-      /\ ![ ^[locals ("rp" :: nil) vs ss st#Sp * sched * M.globalInv * mallocHeap 0] ] st
+      /\ ![ ^[locals ("rp" :: nil) vs ss st#Sp * sched fs * M.globalInv * mallocHeap 0] ] st
       ---> #0 st)%PropX.
 
 Lemma starting_elim : forall specs pc ss P stn st,
   interp specs (![ starting pc ss * P ] (stn, st))
   -> (exists pre, specs pc = Some (fun x => pre x)
     /\ interp specs (![ P ] (stn, st))
-    /\ forall stn_st vs, interp specs ([| stn_st#Sp <> 0 /\ freeable stn_st#Sp (1 + ss) |]
+    /\ forall stn_st vs fs, interp specs ([| stn_st#Sp <> 0 /\ freeable stn_st#Sp (1 + ss) |]
       /\ ![ locals ("rp" :: nil) vs ss stn_st#Sp
-      * sched * M.globalInv * mallocHeap 0 ] stn_st
+      * sched fs * M.globalInv * mallocHeap 0 ] stn_st
     ---> pre stn_st)%PropX).
   cptr.
   generalize (split_semp _ _ _ H0 H); intros; subst; auto.
@@ -91,15 +240,15 @@ Local Hint Resolve split_a_semp_a semp_smem_emp.
 Lemma starting_intro : forall specs pc ss P stn st,
   (exists pre, specs pc = Some (fun x => pre x)
     /\ interp specs (![ P ] (stn, st))
-    /\ forall stn_st vs, interp specs ([| stn_st#Sp <> 0 /\ freeable stn_st#Sp (1 + ss) |]
+    /\ forall stn_st vs fs, interp specs ([| stn_st#Sp <> 0 /\ freeable stn_st#Sp (1 + ss) |]
       /\ ![ locals ("rp" :: nil) vs ss stn_st#Sp
-      * sched * M.globalInv * mallocHeap 0 ] stn_st
+      * sched fs * M.globalInv * mallocHeap 0 ] stn_st
     ---> pre stn_st)%PropX)
   -> interp specs (![ starting pc ss * P ] (stn, st)).
   cptr.
 Qed.
 
-Lemma other_starting_intro : forall specs ts w pc ss P stn st,
+(*Lemma other_starting_intro : forall specs ts w pc ss P stn st,
   (exists pre, specs pc = Some (fun x => pre x)
     /\ interp specs (![ P ] (stn, st))
     /\ forall stn_st vs ts' w', interp specs ([| ts %<= ts' |]
@@ -110,36 +259,86 @@ Lemma other_starting_intro : forall specs ts w pc ss P stn st,
     ---> pre stn_st)%PropX)
   -> interp specs (![ Q'.starting ts w pc ss * P ] (stn, st)).
   cptr.
-Qed.
+Qed.*)
 
 
 Local Notation "'PREexit' [ vs ] pre" := (Q'.Q.localsInvariantExit (fun vs _ => pre%qspec%Sep))
   (at level 89).
 
-Definition initS : spec := SPEC reserving 16
+Definition initS : spec := SPEC reserving 18
   PRE[_] globalSched =?> 1 * mallocHeap 0
-  POST[R] sched * mallocHeap 0.
+  POST[R] sched empty * mallocHeap 0.
 
 Definition spawnS : spec := SPEC("pc", "ss") reserving 25
-  PRE[V] [| V "ss" >= $2 |] * sched * starting (V "pc") (wordToNat (V "ss") - 1) * mallocHeap 0
-  POST[_] sched * mallocHeap 0.
+  Al fs,
+  PRE[V] [| V "ss" >= $2 |] * sched fs * starting (V "pc") (wordToNat (V "ss") - 1) * mallocHeap 0
+  POST[_] sched fs * mallocHeap 0.
 
 Definition exitS : spec := SPEC("sc", "ss") reserving 2
-  PREexit[V] [| V "ss" >= $3 |] * sched * M.globalInv * mallocHeap 0.
+  Al fs,
+  PREexit[V] [| V "ss" >= $3 |] * sched fs * M.globalInv * mallocHeap 0.
 
 Definition yieldS : spec := SPEC reserving 25
-  PRE[_] sched * M.globalInv * mallocHeap 0
-  POST[_] sched * M.globalInv * mallocHeap 0.
+  Al fs,
+  PRE[_] sched fs * M.globalInv * mallocHeap 0
+  POST[_] Ex fs', [| fs %<= fs' |] * sched fs' * M.globalInv * mallocHeap 0.
 
-Definition m := bimport [[ "threadqs"!"alloc" @ [Q'.allocS], "threadqs"!"spawn" @ [Q'.spawnS],
+Definition initSize := 2.
+
+Theorem initSize_eq : initSize = 2.
+  auto.
+Qed.
+
+Opaque initSize.
+
+Definition m := bimport [[ "malloc"!"malloc" @ [mallocS], "malloc"!"free" @ [freeS],
+                           "threadqs"!"alloc" @ [Q'.allocS], "threadqs"!"spawn" @ [Q'.spawnS],
                            "threadqs"!"exit" @ [Q'.exitS], "threadqs"!"yield" @ [Q'.yieldS] ]]
   bmodule "scheduler" {{
-    bfunction "init"() [initS]
-      $[globalSched] <-- Call "threadqs"!"alloc"()
-      [PRE[_, R] globalSched =?> 1
-       POST[_] globalSched =*> R];;
+    bfunction "init"("root", "ready", "wait") [initS]
+      "root" <-- Call "malloc"!"malloc"(0, 4)
+      [PRE[_, R] globalSched =?> 1 * R =?> 4 * mallocHeap 0
+       POST[_] sched empty * mallocHeap 0];;
+
+      globalSched *<- "root";;
+
+      Assert [PRE[V] globalSched =*> V "root" * V "root" =?> 4 * mallocHeap 0 * tqs empty empty
+        POST[_] sched empty * mallocHeap 0];;
+
+      "ready" <-- Call "threadqs"!"alloc"()
+      [PRE[V, R] globalSched =*> V "root" * V "root" =?> 4 * tqs (empty %+ R) empty * mallocHeap 0
+       POST[_] sched empty * mallocHeap 0];;
+
+      "wait" <-- Call "malloc"!"malloc"(0, initSize)
+      [PRE[V, R] R =?> initSize * [| R <> 0 |] * [| freeable R initSize |]
+         * globalSched =*> V "root" * V "root" =?> 4
+         * tqs (empty %+ V "ready") empty
+       POST[_] sched empty];;
+
+      Note [make_array initSize];;
+
+      Assert [Al waitL,
+        PRE[V] array waitL (V "wait") * [| length waitL = 2 |] * [| V "wait" <> 0 |] * [| freeable (V "wait") 2 |]
+          * [| ($0 < natToW (length waitL))%word |]
+          * globalSched =*> V "root" * V "root" =?> 4 * tqs (empty %+ V "ready") empty
+        POST[_] sched empty];;
+
+      "wait"+0 *<- 0;;
+
+      Assert [Al waitL,
+        PRE[V] array waitL (V "wait") * [| length waitL = 2 |] * [| V "wait" <> 0 |] * [| freeable (V "wait") 2 |]
+          * [| ($1 < natToW (length waitL))%word |] * [| Array.selN waitL 0 = $0 |]
+          * globalSched =*> V "root" * V "root" =?> 4 * tqs (empty %+ V "ready") empty
+        POST[_] sched empty];;
+
+      "wait"+4 *<- 0;;
+
+      "root" *<- "ready";;
+      "root"+4 *<- 0;;
+      "root"+8 *<- "wait";;
+      "root"+12 *<- 2;;
       Return 0
-    end with bfunction "spawn"("pc", "ss") [spawnS]
+    end (*with bfunction "spawn"("pc", "ss") [spawnS]
       Call "threadqs"!"spawn"($[globalSched], "pc", "ss")
       [PRE[_] Emp
        POST[_] Emp];;
@@ -152,13 +351,53 @@ Definition m := bimport [[ "threadqs"!"alloc" @ [Q'.allocS], "threadqs"!"spawn" 
       [PRE[_] Emp
        POST[_] Emp];;
       Return 0
-    end
+    end*)
   }}.
 
-Ltac t := abstract (unfold globalInv; sep hints; auto).
+Ltac finish := auto;
+  try solve [ try rewrite initSize_eq in *;
+    repeat match goal with
+             | [ H : _ = _ |- _ ] => rewrite H
+           end; reflexivity || auto 2 ].
+
+Lemma selN_updN_eq : forall v a n,
+  (n < length a)%nat
+  -> Array.selN (Array.updN a n v) n = v.
+  induction a; destruct n; simpl; intuition.
+Qed.
+
+Lemma selN_upd_eq : forall v a n,
+  (n < length a)%nat
+  -> goodSize (length a)
+  -> Array.selN (Array.upd a (natToW n) v) n = v.
+  intros; rewrite upd_updN.
+  apply selN_updN_eq; auto.
+  eauto using goodSize_weaken.
+Qed.
+
+Local Hint Extern 1 (selN _ _ = _) => apply selN_upd_eq; solve [ finish ].
+
+(*Ltac t := abstract (unfold globalInv; sep hints; auto).*)
+Ltac t := solve [ unfold globalInv; sep hints; finish ].
 
 Local Hint Extern 1 (@eq W _ _) => words.
 Local Hint Immediate evolve_refl.
+
+Hint Rewrite upd_length : sepFormula.
+
+Local Hint Unfold allIn allInOrZero.
+
+Local Hint Extern 1 (List.Forall _ (Array.upd _ (natToW 1) (natToW 0))) =>
+  rewrite upd_updN by auto;
+    repeat match goal with
+             | [ ls : list W |- _ ] =>
+               match goal with
+                 | [ _ : length ?E = _ |- _ ] =>
+                   match E with
+                     | context[ls] => destruct ls; try discriminate
+                   end
+               end
+           end; simpl in *.
 
 Theorem ok : moduleOk m.
   vcgen.
@@ -167,7 +406,24 @@ Theorem ok : moduleOk m.
   t.
   t.
   t.
+  t.
+  t.
+  t.
+  t.
+  t.
+  t.
+  t.
+  t.
+  t.
+  t.
+  t.
+  t.
+  t.
+  t.
+  t.
+  t.
 
+(*
   post; evaluate auto_ext.
   match goal with
     | [ H : interp ?specs (![?P] ?x) |- _ ] =>
@@ -270,6 +526,9 @@ Theorem ok : moduleOk m.
   t.
   t.
   t.
+*)
 Qed.
+
+Transparent initSize.
 
 End Make.
